\begin{align}
  \begin{Bmatrix}a : k_{f}, & b : - Y k_{f} - Z k_{f} - k_{b}, & c : Y Z k_{f}\end{Bmatrix} \\
  P = \sqrt{- 4 a c + b^{2}} \\
  \frac{1}{P} \left(- \log{\left (\frac{- P + b}{P + b} \right )} + \log{\left (\frac{- P + 2 a x + b}{P + 2 a x + b} \right )}\right) = t \\
  x = \frac{\left(P - b\right) \left(- P e^{P t} + P - b e^{P t} + b\right)}{2 a \left(P + b + \left(P - b\right) e^{P t}\right)} \\
  Q = P + b \\
  R = P - b \\
  x = - \frac{Q \left(e^{P t} - 1\right)}{2 a \left(\frac{Q}{R} + e^{P t}\right)}
\end{align}
