\begin{align}
  \frac{d}{d t} x = Y k_{f} \left(Z - x\right) - k_{b} x \\
  \int_{0}^{x} \frac{1}{Y k_{f} \left(Z - \chi\right) - \chi k_{b}}\, d\chi = \int_{0}^{t} 1\, d\tau \\
  \frac{1}{Y k_{f} + k_{b}} \left(\log{\left (- Y Z k_{f} \right )} - \log{\left (- Y Z k_{f} + x \left(Y k_{f} + k_{b}\right) \right )}\right) = t \\
  x = \frac{Y Z k_{f} \left(e^{t \left(Y k_{f} + k_{b}\right)} - 1\right)}{\left(Y k_{f} + k_{b}\right) e^{t \left(Y k_{f} + k_{b}\right)}} \\
  x = \frac{Y Z k_{f}}{Y k_{f} + k_{b}} \left(1 - e^{- t \left(Y k_{f} + k_{b}\right)}\right)
\end{align}
