\begin{align}
  \frac{d}{d t} x = k'_{f} \left(Z - x\right) - k_{b} x \\
  \int_{0}^{x} \frac{1}{- \chi k_{b} + k'_{f} \left(Z - \chi\right)}\, d\chi = \int_{0}^{t} 1\, d\tau \\
  \frac{1}{k'_{f} + k_{b}} \left(\log{\left (- Z k'_{f} \right )} - \log{\left (- Z k'_{f} + x \left(k'_{f} + k_{b}\right) \right )}\right) = t \\
  x = \frac{Z k'_{f} \left(e^{t \left(k'_{f} + k_{b}\right)} - 1\right)}{\left(k'_{f} + k_{b}\right) e^{t \left(k'_{f} + k_{b}\right)}} \\
  x = \frac{Z k'_{f}}{k'_{f} + k_{b}} \left(1 - e^{- t \left(k'_{f} + k_{b}\right)}\right)
\end{align}